Publish previews: main ba52c1c5, 8 PRs, 2 unavailable
Main: ba52c1c5

Pull requests:
- PR #181: published at 7e02bb1d (9 changed variants)
- PR #185: published at b7729749 (9 changed variants)
- PR #203: published at f7a57a2d (9 changed variants)
- PR #216: published at 6be73180 (9 changed variants)
- PR #230: published at ccdf0d3e (9 changed variants)
- PR #231: published at 152e9d04 (9 changed variants)
- PR #244: published at b4a05327 (9 changed variants)
- PR #245: published at a9d376a9 (9 changed variants)
- PR #247: ci-failed at 5f2ee5de
- PR #250: ci-failed at 5b9541bc

pr/203/head/hl/student/html-multi/-verso-search/searchIndex_149.8a4beb2877cc3b88.js
@@ -1,0 +1,1 @@
+window.docContents[149].resolve({"/Equiv/#Equiv":{"contents":"open scoped MyGetElem\n\n\n\n\n\n\n\n\n\n\n","context":"Hoare Logic","header":"4. Equiv: Program Equivalence","id":"/Equiv/#Equiv"}});
