pr/203/head/hl/solutions/lean/HL.lean
@@ -1,3 +1,5 @@
 import HL.Preface
 import HL.Slang
 import HL.Imp
+import HL.Equiv
+import HL.Hoare
