pr/203/head/hl/student/lean/HL/Equiv.lean
@@ -1,0 +1,456 @@
+import LF.Typeclasses
+import HL.Imp
+
+import HL.SFLCompat
+
+-- # Equiv: Program Equivalence
+
+open scoped MyGetElem
+
+-- ## Behavioral Equivaleence
+
+-- In an earlier chapter, we investigated the correctness of a very simple
+-- program transformation: the `optimize_0plus` function. The programming
+-- language we were considering was the first version of the language of
+-- arithmetic expressions -- with no variables -- so in that setting it was
+-- very easy to define what it means for a program transformation to be
+-- correct: it should always yield a program that evaluates to the same number
+-- as the original.
+
+-- To talk about the correctness of program transformations for the full Imp
+-- language -- in particular, assignment -- we need to consider the role of
+-- mutable state and develop a more sophisticated notion of correctness, which
+-- we'll call *behavioral equivalence*.
+
+-- For example:
+
+-- - `X + 2` is behaviorally equivalent to `1 + X + 1`
+-- - `X - X` is behaviorally equivalent to `0`
+-- - `(X - 1) + 1` is *not* behaviorally equivalent to `X`
+
+-- ### Definitions
+
+-- For `aexp`s and `bexp`s with variables, the definition we want is clear:
+-- Two `aexp`s or `bexp`s are "behaviorally equivalent" if they evaluate to
+-- the same result in every state.
+
+def Aexp.equiv (a₁ a₂ : Aexp) : Prop :=
+  ∀ (st: State),
+    a₁.eval st = a₂.eval st
+
+def Bexp.equiv (b₁ b₂ : Bexp) : Prop :=
+  ∀ (st: State),
+    b₁.eval st = b₂.eval st
+
+-- -- ::::full -- Here are some simple examples of equivalences of arithmetic
+-- -- and boolean expressions. -- ::::
+
+example : Aexp.equiv
+          (aexp { X - X })
+          (aexp { 0 }) :=
+  by
+    intros st
+    simp
+
+example : Bexp.equiv
+          (bexp { X - X = 0 })
+          (bexp { true }) :=
+  by
+    intros st
+    simp
+
+-- For commands, the situation is a little more subtle. We can't simply say
+-- "two commands are behaviorally equivalent if they evaluate to the same
+-- ending state whenever they are started in the same initial state," because
+-- some commands, when run in some starting states, don't terminate in any
+-- final state at all!
+
+-- What we need instead is this: two commands are behaviorally equivalent if,
+-- for any given starting state, they either (1) both diverge or else (2) both
+-- terminate in the same final state. A compact way to express this is "if the
+-- first one terminates in a particular state then so does the second, and
+-- vice versa."
+
+def Com.equiv (c₁ c₂: Com) : Prop :=
+    ∀ (st st': State),
+      (st =[ c₁ ]=> st') ↔ (st =[ c₂ ]=> st')
+
+-- ### Simple Examples
+
+-- For examples of command equivalence, let's start by looking at a trivial
+-- equivalence involving `skip`.
+
+theorem skip_left: ∀ c,
+  Com.equiv
+    (imp { skip; ~c })
+    c := by
+  all_goals
+    intros c st st'
+    constructor <;> intro h
+    case mp =>
+      cases h with
+      | seq _ _ _ _ _ h1 h2 =>
+        cases h1 with
+        | skip => assumption
+    case mpr =>
+      apply Com.EvalR.seq _ _ _ st
+      · apply Com.EvalR.skip
+      · assumption
+
+-- ### Exercise (2 stars): skip_right ⭐⭐
+
+-- Prove that adding a `skip` *after* a command also results in an equivalent
+-- program.
+
+theorem skip_right : ∀ c,
+  Com.equiv
+    (imp { ~c  skip; })
+    c := by
+  sorry
+
+-- Similarly, here is a simple equivalence that optimises `if` commands.
+
+theorem if_true_simple: ∀ c₁ c₂,
+  Com.equiv
+    (imp {if (true) {~c₁} else {~c₂}})
+    c₁ := by
+  intro c₁ c₂ st st'
+  constructor <;> intro h
+  case mp =>
+    cases h with
+    | ifTrue => assumption
+    | ifFalse => contradiction
+  case mpr =>
+    apply Com.EvalR.ifTrue
+    · rfl
+    · assumption
+
+-- Of course, no programmer would write a conditional whose condition is
+-- literally `true`. (At least, no human programmer -- compilers and macro
+-- preprocessors do this sort of thing internally all the time!) But they
+-- might write one whose condition is *equivalent* to true:
+
+-- *Theorem*: If `b` is equivalent to `true`, then `if (~b) {~c₁}
+-- else {~c₂}`
+-- is equivalent to `c₁`. *Proof*:
+
+-- - (`->`) We must show, for all `st` and `st'`, that if
+--   `st =[ imp {if (~b) {~c₁} else {~c₂}} ]=> st'` then `st =[ c₁ ]=> st'`.
+
+--   Proceed by cases on the rules that could possibly have been used to show
+--   `st =[ imp {if (~b) {~c₁} else {~c₂}} ]=> st'`, namely `Com.EvalR.ifTrue`
+--   and `Com.EvalR.ifFalse`.
+
+--   - Suppose the final rule in the derivation of
+--     `st =[ imp {if (~b) {~c₁} else {~c₂}} ]=> st'` was `Com.EvalR.ifTrue`. We
+--     then have, by the premises of `Com.EvalR.ifTrue`, that `st =[ c₁ ]=> st'`.
+--     This is exactly what we set out to prove.
+
+--   - On the other hand, suppose the final rule in the derivation of
+--     `st =[ imp {if (~b) {~c₁} else {~c₂}} ]=> st'` was `Com.EvalR.ifFalse`. We
+--     then know that `b.eval st = false` and `st =[ c₂ ]=> st'`.
+
+--     Recall that `b` is equivalent to `true`, i.e., forall `st`,
+--     `b.eval st = (bexp {true}).eval st`. In particular, this means that
+--     `b.eval st = true`, since `(bexp {true}).eval st = true`. But this is a
+--     contradiction, since `Com.EvalR.ifFalse` requires that `b.eval st = false`.
+--     Thus, the final rule could not have been `Com.EvalR.ifFalse`.
+
+-- - (`<-`) We must show, for all `st` and `st'`, that if `st =[ c₁ ]=> st'`
+--   then `st =[ imp {if (~b) {~c₁} else {~c₂}} ]=> st'`.
+
+--   Since `b` is equivalent to `true`, we know that `b.eval st` =
+--   `(bexp {true}).eval st = true` = `true`. Together with the assumption that
+--   `st =[ c₁ ]=> st'`, we can apply `Com.EvalR.ifTrue` to derive
+--   `st =[ imp {if (~b) {~c₁} else {~c₂}} ]=> st'`.
+
+-- Here is the formal version of this proof:
+
+theorem if_true_equiv: ∀ b c₁ c₂,
+  Bexp.equiv b (bexp {true}) ->
+  Com.equiv
+    (imp {if (~b) {~c₁} else {~c₂}})
+    c₁ := by
+  intro b c₁ c₂ hb st st'
+  constructor <;> intro h
+  case mp =>
+    cases h with
+    | ifTrue => assumption
+    | ifFalse _ _ _ _ _ hb' hc =>
+      unfold Bexp.equiv at hb; simp at hb
+      rw [hb] at hb'
+      contradiction
+  case mpr =>
+    apply Com.EvalR.ifTrue <;> try assumption
+    unfold Bexp.equiv at hb; dsimp at hb
+    apply hb
+
+-- ### Exercise (2 stars): if_false_equiv ⭐⭐
+
+theorem if_false_equiv: ∀ b c₁ c₂,
+  Bexp.equiv b (bexp {false}) ->
+  Com.equiv
+    (imp {if (~b) {~c₁} else {~c₂}})
+    c₂ := by
+  sorry
+
+-- ### Exercise (3 stars): swap_if_branches ⭐⭐⭐
+
+-- Show that we can swap the branches of an `if` if we also negate its
+-- condition.
+
+theorem swap_if_branches : ∀ b c₁ c₂,
+  Com.equiv
+    (imp {if (~b) {~c₁} else {~c₂}})
+    (imp {if (¬ ~b) {~c₂} else {~c₁}}) := by
+  sorry
+
+-- For `while` loops, we can give a similar pair of theorems. A loop whose
+-- guard is equivalent to `false` is equivalent to `skip`, while a loop whose
+-- guard is equivalent to `true` is equivalent to `while (true) {skip;} end`
+-- (or any other non-terminating program).
+
+-- The first of these facts is easy.
+
+theorem while_false_equiv : ∀ b c,
+  Bexp.equiv b (bexp {false}) ->
+  Com.equiv
+    (imp {while (~b) {~c}})
+    (imp {skip;}) := by
+  intro b c hb st st'
+  constructor <;> intro h
+  case mp =>
+    cases h with
+    | whileFalse => apply Com.EvalR.skip
+    | whileTrue _ _ _ _ _ hb' hc hloop =>
+      rw [hb] at hb'
+      simp at hb'
+  case mpr =>
+    cases h with
+    | skip =>
+      apply Com.EvalR.whileFalse
+      apply hb
+
+-- ### Exercise (2 stars): while_false_informal (Advanced, manually graded) ⭐⭐
+
+-- Write an informal proof of `while_false_equiv`.
+
+-- To prove the second fact, we need an auxiliary lemma stating that `while`
+-- loops whose guards are equivalent to `true` never terminate.
+
+-- *Lemma*: If `b` is equivalent to `true`, then it cannot be the case that
+-- `st =[ while (~b) {~c} ]=> st'`.
+
+-- *Proof*: Suppose that `st =[ while (~b) {~c} ]=> st'`. We show, by
+-- induction on a derivation of `st =[ while (~b) {~c} ]=> st'`, that this
+-- assumption leads to a contradiction. The only two cases to consider are
+-- `Com.EvalR.whileFalse` and `Com.EvalR.whileTrue`; the others are
+-- contradictory.
+
+-- - Suppose `st =[ while (~b) {~c} ]=> st'` is proved using rule
+--   `Com.EvalR.whileFalse`. Then by assumption `b.eval st = false`. But this
+--   contradicts the assumption that `b` is equivalent to `true`.
+
+-- - Suppose `st =[ while (~b) {~c} ]=> st'` is proved using rule
+--   `Com.EvalR.whileTrue`. We must have:
+
+--   1. `b.eval st = true`, and
+
+--   2. there is some `st₀` such that `st =[ c ] => st₀` and
+--      `st₀ =[ while (~b) {~c} ]=> st'`.
+
+--   3. Also, we are given an induction hypothesis saying that
+--      `st₀ =[ while (~b) {~c} ]=> st'` leads to a contradiction,
+
+--   We obtain a contradiction by 2 and 3.
+
+theorem while_true_nonterm : ∀ b c st st',
+  Bexp.equiv b (bexp {true}) ->
+  ¬ (st =[ while (~b) {~c} ]=> st') := by
+  all_goals
+    intro b c st st' hb contra
+    have key : ∀ (c': Com) (s s': State), (s =[ c' ]=> s') -> c' = (imp {while (~b) {~c}}) -> False :=
+      by
+        intro c' s s' hce
+        induction hce with
+        | whileFalse b' s0 c0 hb' =>
+          intro heq; injection heq with beq ceq
+          subst beq; rw [hb] at hb'
+          simp at hb'
+        | whileTrue s0 s0' s0'' b' c0 hb hc' hwhile ih1 ih2 => exact ih2
+        | skip => simp
+        | asgn => simp
+        | seq => simp
+        | ifTrue => simp
+        | ifFalse => simp
+    exact key (imp {while (~b) {~c}}) st st' contra (by rfl)
+
+-- ### Exercise (2 stars): while_true_nonterm_informal (manually graded) ⭐⭐
+
+-- Explain what the lemma `while_true_nonterm` means in English.
+
+-- ### Exercise (2 stars): while_true ⭐⭐
+
+-- Prove the following theorem. *Hint*: You'll want to use
+-- `while_true_nonterm` here.
+
+theorem while_true : ∀ b c,
+  Bexp.equiv b (bexp {true}) ->
+  Com.equiv
+    (imp {while (~b) {~c}})
+    (imp {while (true) {skip;}}) := by
+  sorry
+
+-- A more interesting fact about `while` commands is that any number of copies
+-- of the body can be "unrolled" without changing meaning.
+
+-- Loop unrolling is an important transformation in any real compiler, so its
+-- correctness is of more than just academic interest!
+
+theorem loop_unrolling : ∀ b c,
+  Com.equiv
+    (imp {while (~b) {~c}})
+    (imp {
+      if (~b) {~c} else {skip;}
+      while (~b) {~c}
+    }) := by
+  all_goals
+    intro b c st st'
+    constructor <;> intro hce
+    case mp =>
+      cases hce with
+      | whileFalse _ _ _ hb =>
+        apply Com.EvalR.seq _ _ _ st
+        · apply Com.EvalR.ifFalse <;> try assumption
+          apply Com.EvalR.skip
+        · apply Com.EvalR.whileFalse <;> try assumption
+      | whileTrue _ st'' _ _ _ hb hc hloop =>
+        apply Com.EvalR.seq _ _ _ st''
+        · apply Com.EvalR.ifTrue <;> try assumption
+        · assumption
+    case mpr =>
+      cases hce with
+      | seq _ _ _ st'' _ h1 h2 =>
+        cases h1 with
+        | ifTrue _ _ _ _ _ hb hc =>
+          apply Com.EvalR.whileTrue _ st'' <;> try assumption
+        | ifFalse _ _ _ _ _ hb hc =>
+          cases hc with
+          | skip => assumption
+
+-- Proving program properties involving assignments is one place where the
+-- fact that we are treating equality on program states extensionally (e.g.,
+-- `x →ₜ m[x] ; m` and `m` are equal maps) comes in handy.
+
+theorem identity_assignment : ∀ X,
+  Com.equiv
+    (imp {X := X;})
+    (imp {skip;}) := by
+  intro X st st'
+  constructor <;> intro hce
+  case mp =>
+    cases hce with
+    | asgn _ _ n _ h =>
+      dsimp at h
+      rw [← h, TotalMap.update_same]
+      apply Com.EvalR.skip
+
+  case mpr =>
+    cases hce with
+    | skip =>
+      suffices st =[ X := X; ]=> X →ₜ st[X] ; st by
+        simp only [TotalMap.update_same] at this
+        exact this
+      apply Com.EvalR.asgn
+      simp
+
+-- ### Exercise (2 stars): assign_equiv ⭐⭐
+
+theorem assign_equiv : ∀ (X : Ident) (a : Aexp),
+  Aexp.equiv (aexp {X}) a ->
+  Com.equiv
+    (imp {skip;})
+    (imp {X := ~a;}) := by
+  sorry
+
+-- ## Properties of Behavior Equivalence
+
+-- We next consider some fundamental properties of program equivalence.
+
+-- ### Behavioral Equivalence is an Equivalence
+
+-- First, let's verify that the equivalences on `Aexp`s, `Bexp`s, and `Com`s
+-- really are *equivalences* -- ie, that they are reflexive, symmetric, and
+-- transitive. These proofs are all easy.
+
+theorem Aexp.equiv.refl : ∀ (a : Aexp),
+  a.equiv a := by
+  intros a st
+  rfl
+
+theorem Aexp.equiv.sym : ∀ (a₁ a₂ : Aexp),
+  a₁.equiv a₂ → a₂.equiv a₁ := by
+  intro a₁ a₂ h st
+  rw [h]
+
+theorem Aexp.equiv.trans : ∀ (a₁ a₂ a₂ : Aexp),
+  a₁.equiv a₂ → a₂.equiv a₃ → a₁.equiv a₃ := by
+  intro a₁ a₂ a₃ h₁ h₂ st
+  rw [h₁, h₂]
+
+theorem Bexp.equiv.refl : ∀ (b : Bexp),
+  b.equiv b := by
+  intros b st
+  rfl
+
+theorem Bexp.equiv.sym : ∀ (b₁ b₂ : Bexp),
+  b₁.equiv b₂ → b₂.equiv b₁ := by
+  intro b₁ b₂ h st
+  rw [h]
+
+theorem Bexp.equiv.trans : ∀ (b₁ b₂ b₂ : Bexp),
+  b₁.equiv b₂ → b₂.equiv b₃ → b₁.equiv b₃ := by
+  intro b₁ b₂ b₃ h₁ h₂ st
+  rw [h₁, h₂]
+
+theorem Com.equiv.refl : ∀ (c : Com),
+  c.equiv c := by
+  intros c st st'
+  rfl
+
+theorem Com.equiv.sym : ∀ (c₁ c₂ : Com),
+  c₁.equiv c₂ → c₂.equiv c₁ := by
+  intro c₁ c₂ h st st'
+  rw [h]
+
+theorem Com.equiv.trans : ∀ (c₁ c₂ c₂ : Com),
+  c₁.equiv c₂ → c₂.equiv c₃ → c₁.equiv c₃ := by
+  intro c₁ c₂ c₃ h₁ h₂ st st'
+  rw [h₁, h₂]
+
+-- ### Behavioral Equivalence is a Congruence
+
+-- Less obviously, behavioral equivalence is also a *congruence*. That is, the
+-- equivalence of two subprograms implies the equivalence of the larger
+-- programs in which they are embedded:
+
+-- aequiv a a' ------------------------- cequiv (x := a) (x := a')
+
+-- cequiv c1 c1' cequiv c2 c2' -------------------------- cequiv (c1;c2)
+-- (c1';c2')
+
+-- ... and so on for the other forms of commands.
+
+-- (Note that we are using the inference rule notation here not as part of an
+-- inductive definition, but simply to write down some valid implications in a
+-- readable format. We prove these implications below.)
+
+-- We will see a concrete example of why these congruence properties are
+-- important in the following section (in the proof of
+-- `fold_constants_com_sound`), but the main idea is that they allow us to
+-- replace a small part of a large program with an equivalent small part and
+-- know that the whole large programs are equivalent *without* doing an
+-- explicit proof about the parts that didn't change -- i.e., the "proof
+-- burden" of a small change to a large program is proportional to the size of
+-- the change, not the program!
+
