pr/203/head/lf/student/lean/LF/Preface.lean
@@ -4,16 +4,16 @@ import LF.SFLCompat
 
 -- ## Welcome
 
--- This is the entry point to a series of electronic textbooks on various
--- aspects of *Software Foundations*, the mathematical underpinnings of
--- reliable software. Topics in the series include basic concepts of logic,
--- functional programming, computer-assisted theorem proving, operational
--- semantics, logics and techniques for reasoning about programs, static type
--- systems, property-based random testing, and verification of practical C
--- code. The exposition is intended for a broad range of readers, from
--- advanced undergraduates to PhD students and researchers. No specific
--- background in logic or programming languages is assumed, though a degree of
--- mathematical maturity will be helpful.
+-- This is the starting point for a series of electronic textbooks on
+-- *Software Foundations*, the mathematical underpinnings of reliable
+-- software. Topics in the series include basic concepts of logic, functional
+-- programming, computer-assisted theorem proving, operational semantics,
+-- logics and techniques for reasoning about programs, static type systems,
+-- property-based random testing, and verification of practical C code. The
+-- exposition is intended for a broad range of readers, from advanced
+-- undergraduates to PhD students and researchers. No specific background in
+-- logic or programming languages is assumed, though a degree of mathematical
+-- maturity will be helpful.
 
 -- The principal novelty of the series is that it is one hundred percent
 -- formalized and machine-checked: each text is literally a script for Lean.
@@ -60,14 +60,13 @@ import LF.SFLCompat
 -- Logic is the field of study whose subject matter is *proofs* --
 -- unassailable arguments for the truth of particular propositions. Volumes
 -- have been written about the central role of logic in computer science.
--- Manna and Waldinger called it "the calculus of computer science," while
--- Halpern et al.'s paper *On the Unusual Effectiveness of Logic in Computer
--- Science* catalogs scores of ways in which logic offers critical tools and
--- insights. Indeed, they observe that, "As a matter of fact, logic has turned
--- out to be significantly more effective in computer science than it has been
--- in mathematics. This is quite remarkable, especially since much of the
--- impetus for the development of logic during the past one hundred years came
--- from mathematics."
+-- called it "the calculus of computer science," while 's paper *On the
+-- Unusual Effectiveness of Logic in Computer Science* catalogs scores of ways
+-- in which logic offers critical tools and insights. Indeed, they observe
+-- that, "As a matter of fact, logic has turned out to be significantly more
+-- effective in computer science than it has been in mathematics. This is
+-- quite remarkable, especially since much of the impetus for the development
+-- of logic during the past one hundred years came from mathematics."
 
 -- In particular, the fundamental tools of *inductive proof* are ubiquitous
 -- across computer science. You have surely seen them before, perhaps in a
@@ -108,19 +107,22 @@ import LF.SFLCompat
 -- semi-automatically, and a highly extensible system for defining new
 -- proof-automation tactics and notations for specific situations.
 
--- Lean and its relatives have become a critical enablers for a huge variety
--- of work across computer science and mathematics:
+-- Lean and its relatives have become critical enablers for a [huge variety of
+-- work](https://leanprover-community.github.io/papers.html) across computer
+-- science and mathematics:
 
--- - As a *platform for modeling programming languages*, they have become
---   standard tools for researchers who need to describe and reason about
+-- - As a *platform for modeling programming languages*, proof assistants have
+--   become standard tools for researchers who need to describe and reason about
 --   complex language definitions. They have been used, for example, to check
 --   the security of the JavaCard platform, obtaining the highest level of
 --   common criteria certification, and for formal specifications of the x86 and
 --   LLVM instruction sets and programming languages such as C.
 
 -- - As *environments for developing formally certified software and hardware*,
---   they been used, for example, to build CompCert, a fully-verified optimizing
---   compiler for C, and CertiKOS, a fully verified hypervisor, for proving the
+--   they have been used, for example, to build CompCert, a fully-verified
+--   optimizing compiler for C,
+--   [Cedar](https://github.com/cedar-policy/cedar-spec), a formally-specified
+--   policy language, and CertiKOS, a fully verified hypervisor, for proving the
 --   correctness of subtle algorithms involving floating point numbers, and as
 --   the basis for CertiCrypt, FCF, and SSProve, which are frameworks for
 --   proving cryptographic algorithms secure. They are also being used to build
@@ -134,14 +136,19 @@ import LF.SFLCompat
 --   checking a large number of configurations using a program. More recently,
 --   an even more massive effort led to a formalization of the Feit-Thompson
 --   Theorem, the first major step in the classification of finite simple
---   groups.
+--   groups. Specifically, Lean is currently at the core of various
+--   formalization efforts in mathematics, such as the proof of [Fermat's Last
+--   Theorem](https://github.com/ImperialCollegeLondon/FLT), the [Sphere Packing
+--   Problem](https://github.com/thefundamentaltheor3m/Sphere-Packing-Lean). and
+--   even DeepMind's AI model for IMO problems
+--   [AlphaProof](https://deepmind.google/blog/ai-solves-imo-problems-at-silver-medal-level/).
 
 -- ### Functional Programming
 
 -- *Functional programming* refers both to a collection of idioms that can be
 -- used in almost any programming language and to a family of languages
 -- designed to foreground these idioms, including Haskell, OCaml, Standard ML,
--- F##, Scala, Scheme, Racket, Common Lisp, Clojure, Erlang, F*, and Lean
+-- F#, Scala, Scheme, Racket, Common Lisp, Clojure, Erlang, F*, and Lean
 -- itself.
 
 -- Functional programming has been developed over many decades — indeed, its
@@ -187,16 +194,16 @@ import LF.SFLCompat
 
 -- ### Further Reading
 
--- This text is intended to be self contained, but readers looking for a
--- deeper treatment of particular topics will find some suggestions for
--- further reading in the Postscript chapter.
+-- This text is intended to be self contained, but readers looking for
+-- follow-on textbooks or deeper treatments of particular topics will find
+-- some suggestions for further reading in the Postscript chapter.
 
 -- ## Practicalities
 
 -- ### System Requirements
 
 -- Lean runs on Windows, Linux, and MacOS. The files in this book have been
--- tested with Lean version `4.32.0`.
+-- tested with Lean version `4.33.0`.
 
 -- ### Installation
 
@@ -276,8 +283,49 @@ import LF.SFLCompat
 -- the course was offered in Rocq, but the ideas behind the problems are still
 -- relevant.
 
--- ## Acknowledgements
+-- ### Credits
 
--- See `ACKNOWLEDGEMENTS.md` in the [SF-in-Lean git
--- repo](https://github.com/plclub/sf-in-lean).
+-- **Leadership:** Mike Hicks and Benjamin C. Pierce lead the SF-in-Lean
+-- project.
+
+-- **Authors:** The Lean adaptation of *Software Foundations* was created by
+-- Mike Hicks, Benjamin C. Pierce, One An, Roger Burtonpatel, Jonathan Chan,
+-- Harry Goldstein, Niklas Halonen, Chris Henson, Kihong Heo, Yipeng Liu, and
+-- Daniel Sainati,
+
+-- **... with contributions from** Luisa Cicolini, Michael Clarkson, Robert
+-- Joseph, Sati, and Shriya Thakur,
+
+-- **... and gratitude to** David Thrane Christiansen, for helping us
+-- understand the intricacies of Lean's Verso document preparation system.
+
+-- **SF in Rocq:** The first three volumes of *Software Foundations in Lean*
+-- (*Logical Foundations*, *Type Systems*, and *Hoare Logic*) are adapted from
+-- the *Logical Foundations* and *Programming Language Foundations* volumes of
+-- the original *Software Foundations* series, developed from 2008 to 2026 by
+-- a large team of authors and contributors led by Benjamin C. Pierce.
+
+-- The original *Logical Foundations* was written by Benjamin C. Pierce,
+-- Arthur Azevedo de Amorim, Chris Casinghino, Marco Gaboardi, Michael
+-- Greenberg, Cătălin Hriţcu, Vilhelm Sjöberg, and Brent Yorgey, with
+-- contributions from Loris D'Antoni, Andrew W. Appel, Arthur Charguéraud,
+-- Michael Clarkson, Anthony Cowley, Jeffrey Foster, Dmitri Garbuzov, Olek
+-- Gierczak, Michael Hicks, Ranjit Jhala, Ori Lahav, Yishuai Li, Greg
+-- Morrisett, Jennifer Paykin, Mukund Raghothaman, Chung-chieh Shan, Leonid
+-- Spesivtsev, Caleb Stanford, Andrew Tolmach, Philip Wadler, Stephanie
+-- Weirich, Li-Yao Xia, and Steve Zdancewic.
+
+-- The original *Programming Language Foundations* was written by Benjamin C.
+-- Pierce, Arthur Azevedo de Amorim, Chris Casinghino, Marco Gaboardi, Michael
+-- Greenberg, Cătălin Hriţcu, Vilhelm Sjöberg, Andrew Tolmach, and Brent
+-- Yorgey with contributions from Loris D'Antoni, Andrew W. Appel, Arthur
+-- Chargueraud, Michael Clarkson, Anthony Cowley, Jeffrey Foster, Dmitri
+-- Garbuzov, Michael Hicks, Ranjit Jhala, Ori Lahav, Yishuai Li, Greg
+-- Morrisett, Jennifer Paykin, Mukund Raghothaman, Chung-Chieh Shan, Leonid
+-- Spesivtsev, Caleb Stanford, Philip Wadler, Stephanie Weirich, Li-Yao Xia,
+-- and Steve Zdancewic.
+
+-- **Funding:** Development of the original *Software Foundations* series in
+-- Rocq was supported, in part, by the National Science Foundation under the
+-- NSF Expeditions grant 1521523, *The Science of Deep Specification*.
 
